Adapt the library, tests and examples to the simplified effect system
Ports ulib, simple-lib, the test suite, the examples, the book and pulse
to the new computation-type syntax, and switches the compiler's own
effect declarations (`FStarC.Effect`) over to it now that stage0
understands them.

Co-authored-by: Copilot <223556219+Copilot@users.noreply.github.com>

examples/layeredeffects/AlgHeap.fst
@@ -1,16 +1,15 @@
 module AlgHeap
 
-(* Essentially a copy of AlgForAll but using a heap for the state *)
+(* Algebraic heap example, now as a plain free monad rather than a layered effect. *)
 
 open FStar.Tactics.V2
 open FStar.List.Tot
-open FStar.Universe
 module Map = FStar.Map
 
 type loc = int
 type state = Map.t loc int
 
-type empty : Type u#aa =
+type empty =
 
 type op =
   | Read
@@ -18,21 +17,19 @@ type op =
   | Raise
   | Other of int
 
-assume val other_inp : int -> Type u#0
-let op_inp : op -> Type u#0 =
- function
+assume val other_inp : int -> Type
+let op_inp : op -> Type = function
  | Read -> unit
  | Write -> state
  | Raise -> exn
  | Other i -> other_inp i
 
-assume val other_out : int -> Type u#0
-let op_out : op -> Type =
- function
+assume val other_out : int -> Type
+let op_out : op -> Type = function
  | Read -> state
  | Write -> unit
  | Raise -> empty
- | Other i -> other_inp i
+ | Other i -> other_out i
 
 noeq
 type tree0 (a:Type) : Type =
@@ -40,47 +37,23 @@ type tree0 (a:Type) : Type =
   | Op     : op:op -> i:(op_inp op) -> k:(op_out op -> tree0 a) -> tree0 a
 
 type ops = list op
+let sublist (l1 l2 : ops) = forall x. memP x l1 ==> memP x l2
 
 let rec abides #a (labs:ops) (f : tree0 a) : prop =
-  begin match f with
-  | Op a i k ->
-    mem a labs /\ (forall o. abides labs (k o))
+  match f with
+  | Op a i k -> memP a labs /\ (forall o. abides labs (k o))
   | Return _ -> True
-  end
 
-type tree (a:Type u#aa)
-          (labs : list u#0 op)
-  : Type u#aa
-  =
-  r:(tree0 a){abides labs r}
+type tree (a:Type) (labs : ops) : Type = r:(tree0 a){abides labs r}
 
-let rec interp_at (l1 l2 : ops) (l : op)
-  : Lemma (mem l (l1@l2) == (mem l l1 || mem l l2))
-          [SMTPat (mem l (l1@l2))]
-  = match l1 with
-    | [] -> ()
-    | _::l1 -> interp_at l1 l2 l
-
-let sublist (l1 l2 : ops) = forall x. mem x l1 ==> mem x l2
-
-let rec sublist_at
-  (l1 l2 : ops)
+let rec sublist_at (l1 l2 : ops)
   : Lemma (sublist l1 (l1@l2) /\ sublist l2 (l1@l2))
-          [SMTPatOr [[SMTPat (sublist l1 (l1@l2))];
-                     [SMTPat (sublist l2 (l1@l2))]]]
-  = match l1 with
-    | [] -> ()
-    | _::l1 -> sublist_at l1 l2
+          [SMTPatOr [[SMTPat (sublist l1 (l1@l2))]; [SMTPat (sublist l2 (l1@l2))]]]
+  = match l1 with | [] -> () | _::l1 -> sublist_at l1 l2
 
-let sublist_at_self
-  (l : ops)
-  : Lemma (sublist l (l@l))
-          [SMTPat (sublist l (l@l))]
-  = ()
-  
 let rec abides_sublist_nopat #a (l1 l2 : ops) (c : tree0 a)
   : Lemma (requires (abides l1 c) /\ sublist l1 l2)
-          (ensures (abides l2) c)
+          (ensures (abides l2 c))
   = match c with
     | Return _ -> ()
     | Op a i k ->
@@ -94,369 +67,73 @@ let abides_sublist #a (l1 l2 : ops) (c : tree0 a)
           (ensures (abides l2 c))
           [SMTPat (abides l2 c); SMTPat (sublist l1 l2)]
   = abides_sublist_nopat l1 l2 c
-  
-let abides_at_self #a
-  (l : ops)
-  (c : tree0 a)
-  : Lemma (abides (l@l) c <==>  abides l c)
-          [SMTPat (abides (l@l) c)]
-  = (* Trigger some patterns *)
-    assert (sublist l (l@l));
-    assert (sublist (l@l) l)
 
-let abides_app #a (l1 l2 : ops) (c : tree0 a)
-  : Lemma (requires (abides l1 c \/ abides l2 c))
-          (ensures (abides (l1@l2) c))
-          [SMTPat (abides (l1@l2) c)]
-  = sublist_at l1 l2
+let widen #a (#labs1 #labs2 : ops) (c : tree a labs1)
+  : Pure (tree a labs2) (requires sublist labs1 labs2) (ensures fun _ -> True)
+  = c
 
-(* Folding a computation tree *)
+let return_l #a (#labs:ops) (x:a) : tree a labs = Return x
+
 val fold_with (#a #b:_) (#labs : ops)
            (f:tree a labs)
            (v : a -> b)
-           (h: (o:op{mem o labs} -> op_inp o -> (op_out o -> b) -> b))
+           (h: (o:op{o `memP` labs} -> op_inp o -> (op_out o -> b) -> b))
            : b
 let rec fold_with #a #b #labs f v h =
   match f with
   | Return x -> v x
-  | Op act i k ->
-    let k' (o : op_out act) : b =
-       fold_with #_ #_ #labs (k o) v h
-    in
-    h act i k'
+  | Op act i k -> h act i (fun o -> fold_with #_ #_ #labs (k o) v h)
 
-let handler_ty_l (o:op) (b:Type) (labs:ops) =
+let handler_tree_op (o:op) (b:Type) (labs:ops) =
   op_inp o -> (op_out o -> tree b labs) -> tree b labs
+let handler_tree (labs0 : ops) (b:Type) (labs1 : ops) : Type =
+  o:op{o `memP` labs0} -> handler_tree_op o b labs1
 
-let handler_ty (labs0 : ops) (b:Type) (labs1 : ops) : Type =
-  o:op{mem o labs0} -> handler_ty_l o b labs1
-
-(* The most generic handling construct, we use it to implement bind.
-It is actually just a special case of folding. *)
-val handle_with (#a #b:_) (#labs0 #labs1 : ops)
+val handle_tree (#a #b:_) (#labs0 #labs1 : ops)
            (f:tree a labs0)
            (v : a -> tree b labs1)
-           (h: handler_ty labs0 b labs1)
+           (h: handler_tree labs0 b labs1)
            : tree b labs1
-let handle_with f v h = fold_with f v h
+let handle_tree f v h = fold_with f v h
 
-let return (a:Type) (x:a)
-  : tree a []
-  = Return x
-
-let bind (a b : Type)
-  (#labs1 #labs2 : ops)
-  (c : tree a labs1)
-  (f : (x:a -> tree b labs2))
+let return (a:Type) (x:a) : tree a [] = Return x
+let bind (a b : Type) (#labs1 #labs2 : ops) (c : tree a labs1) (f : (x:a -> tree b labs2))
   : Tot (tree b (labs1@labs2))
-  = handle_with #_ #_ #labs1 #(labs1@labs2) c f (fun act i k -> Op act i k)
-  
-let subcomp (a:Type)
-  (labs1 labs2 : ops)
-  (f : tree a labs1)
-  : Pure (tree a labs2)
-         (requires (sublist labs1 labs2))
-         (ensures (fun _ -> True))
-  = f
+  = sublist_at labs1 labs2;
+    handle_tree #_ #_ #labs1 #(labs1@labs2) c f (fun act i k -> Op act i k)
 
-let if_then_else
-  (a : Type)
-  (labs1 labs2 : ops)
-  (f : tree a labs1)
-  (g : tree a labs2)
-  (p : bool)
-  : Type
-  = tree a (labs1@labs2)
+let (let!) #a #b #labs1 #labs2 (m : tree a labs1) (f : a -> tree b labs2)
+  : tree b (labs1@labs2) = bind a b m f
 
-let _get : tree state [Read] = Op Read () Return
-
-let _put (s:state) : tree unit [Write] = Op Write s Return
-
-total // need this for catch!!
-reifiable
-reflectable
-effect {
-  Alg (a:Type) (_:ops)
-  with {repr = tree; return; bind; subcomp; if_then_else}
-}
-
-let get () : Alg state [Read] =
-  Alg?.reflect _get
-
-let lift_pure_eff
- (a:Type)
- (wp : pure_wp a)
- (f : unit -> PURE a wp)
- : Pure (tree a [])
-        (requires (wp (fun _ -> True)))
-        (ensures (fun _ -> True))
- = FStar.Monotonic.Pure.elim_pure_wp_monotonicity wp;
-   Return (f ())
-
-sub_effect PURE ~> Alg = lift_pure_eff
-
-let put (s:state) : Alg unit [Write] =
-  Alg?.reflect (_put s)
-
-let raise #a (e:exn) : Alg a [Raise] =  
-  Alg?.reflect (Op Raise e (fun e -> match e with))
-  // funnily enough, the version below also succeeds from concluding
-  // a==empty under the lambda since the context becomes inconsistent
-  //Alg?.reflect (Op Raise e Return
-
-type rwtree a = tree a [Read;Write]
-
-let tbind : #a:_ -> #b:_ -> rwtree a -> (a -> rwtree b) -> rwtree b = fun c f -> bind _ _ c f
-
-let st_wp0 (a:Type) : Type = state -> (a & state -> prop) -> prop
-
-let st_monotonic #a (w : st_wp0 a) : prop =
-  //forall s0 p1 p2. (forall r. p1 r ==> p2 r) ==> w s0 p1 ==> w s0 p2
-  // ^ this version seems to be less SMT-friendly
-  forall s0 p1 p2. (forall x s1. p1 (x, s1) ==> p2 (x, s1)) ==> w s0 p1 ==> w s0 p2
-
-let st_wp (a:Type) = wp:st_wp0 a{st_monotonic wp}
-
-unfold
-let return_wp #a x : st_wp a = fun s0 p -> p (x, s0)
-
-unfold
-let bind_wp #a #b (w : st_wp a) (wf : a -> st_wp b)
-  : st_wp b
-  = fun s0 p -> w s0 (fun (y, s1) -> wf y s1 p)
-
-unfold
-let read_wp : st_wp state = fun s0 p -> p (s0, s0)
-
-unfold
-let write_wp : state -> st_wp unit = fun s _ p -> p ((), s)
-
-(* Also doable with handlers *)
-let rec interp_as_wp #a (t : rwtree a) : st_wp a =
-  match t with
-  | Return x -> return_wp x
-  | Op Read _ k ->
-    bind_wp read_wp (fun s -> interp_as_wp (k s))
-  | Op Write s k ->
-    bind_wp (write_wp s) (fun (o:unit) -> interp_as_wp (k o))
+let get () : tree state [Read] = Op Read () Return
+let put (s:state) : tree unit [Write] = Op Write s Return
+let raise #a (e:exn) : tree a [Raise] = Op Raise e (fun x -> match x with)
 
 let rec interp_rdwr_tree #a (t : tree a [Read;Write]) (s:state) : Tot (a & state) =
   match t with
   | Return x -> (x, s)
-  | Op Read _ k ->
-    interp_rdwr_tree (k s) s
-  | Op Write s k ->
-    interp_rdwr_tree (k ()) s
+  | Op Read _ k -> interp_rdwr_tree (k s) s
+  | Op Write s k -> interp_rdwr_tree (k ()) s
 
-let interp_as_fun #a (t : rwtree a) : (state -> a & state) =
-  interp_rdwr_tree t
+let interp_as_fun #a (t : tree a [Read;Write]) : state -> a & state = interp_rdwr_tree t
 
-(* Bug: defining this as a FStar.Preorder.preorder
-causes stupid failures ahead *)
-val stronger : (#a:Type) -> st_wp a -> st_wp a -> prop
-let stronger w1 w2 = forall p s. w1 p s ==> w2 p s
+let sel (r:loc) : tree int [Read] =
+  let! h = get () in
+  return_l #_ #[] (Map.sel h r)
 
-let equiv #a (w1 w2 : st_wp a) = w1 `stronger` w2 /\ w2 `stronger` w1
-
-let (<<=) = stronger
-
-val interp_ret (#a:Type) (x:a) : Lemma (return_wp x `stronger` interp_as_wp (Return x))
-let interp_ret x = ()
-
-let wp_is_monotonic #a (wp : st_wp a) : prop =
-  forall p1 p2 s0. (forall x s1. p1 (x, s1) ==> p2 (x, s1)) ==> wp s0 p1 ==> wp s0 p2
-
-let bind_preserves_mon #a #b (wp : st_wp a) (f : a -> st_wp b)
-  : Lemma (requires (wp_is_monotonic wp /\ (forall x. wp_is_monotonic (f x))))
-          (ensures (wp_is_monotonic (bind_wp wp f)))
-  = ()
-
-let rec interp_monotonic #a (c:rwtree a) : Lemma (wp_is_monotonic (interp_as_wp c)) =
-  match c with
-  | Return x -> ()
-  | Op Read _ k ->
-    let aux (x:state) : Lemma (wp_is_monotonic (interp_as_wp (k x))) =
-      interp_monotonic (k x)
-    in
-    Classical.forall_intro aux;
-    bind_preserves_mon read_wp (fun x -> interp_as_wp (k x))
-  | Op Write s k ->
-    let aux (x:unit) : Lemma (wp_is_monotonic (interp_as_wp (k x))) =
-      interp_monotonic (k x)
-    in
-    Classical.forall_intro aux;
-    bind_preserves_mon (write_wp s) (fun x -> interp_as_wp (k x))
-
-let elim_str #a (w1 w2 : st_wp a) (p : (a & state -> prop)) (s0:state)
-  : Lemma (requires (w1 <<= w2))
-          (ensures w1 s0 p ==> w2 s0 p)
-  = ()
-#restart-solver
-#push-options "--z3rlimit_factor 4 --split_queries always"
-(* Takes a while *)
-let rec interp_morph #a #b (c : rwtree a) (f : a -> rwtree b) (p:_) (s0:_)
-  : Lemma (interp_as_wp c s0 (fun (y, s1) -> interp_as_wp (f y) s1 p) == interp_as_wp (tbind c f) s0 p)
-  = match c with
-    | Return x -> ()
-    | Op Read _ k ->
-      let aux (o:state) : Lemma (interp_as_wp (k o) s0 (fun (y, s1) -> interp_as_wp (f y) s1 p)
-                                        == interp_as_wp (tbind (k o) f) s0 p) =
-        interp_morph (k o) f p s0
-      in
-      Classical.forall_intro aux
-
-    | Op Write s k ->
-      let aux (o:unit) : Lemma (interp_as_wp (k o) s (fun (y, s1) -> interp_as_wp (f y) s1 p)
-                                        == interp_as_wp (tbind (k o) f) s p) =
-        interp_morph (k o) f p s
-      in
-      Classical.forall_intro aux
-
-    | _ -> ()  // this branch is unreachable
-#pop-options
-val interp_bind (#a #b:Type)
-  (c : rwtree a) (f : a -> rwtree b)
-  (w1 : st_wp a) (w2 : a -> st_wp b)
-  : Lemma (requires w1 <<= interp_as_wp c /\ (forall x. w2 x <<= interp_as_wp (f x)))
-          (ensures bind_wp w1 w2 `stronger` interp_as_wp (tbind c f))
-let interp_bind #a #b c f w1 w2 =
-  let aux (p: (b & state -> prop)) (s0:state) : Lemma (bind_wp w1 w2 s0 p ==> interp_as_wp (tbind c f) s0 p) =
-    calc (==>) {
-      bind_wp w1 w2 s0 p;
-      ==> {}
-      w1 s0 (fun (y, s1) -> w2 y s1 p);
-      ==> { (* hyp *)}
-      interp_as_wp c s0 (fun (y, s1) -> w2 y s1 p);
-      ==> { interp_monotonic c }
-      interp_as_wp c s0 (fun (y, s1) -> interp_as_wp (f y) s1 p);
-      ==> { interp_morph c f p s0 }
-      interp_as_wp (tbind c f) s0 p;
-    }
-  in
-  Classical.forall_intro_2 aux
-
-let repr (a : Type) (w: st_wp a) =
-  c:(rwtree a){w `stronger` interp_as_wp c}
-
-let return2 (a:Type) (x:a) : repr a (return_wp x) =
-  interp_ret x;
-  Return x
-
-let bind2 (a : Type) (b : Type)
-  (wp_v : st_wp a) (wp_f: a -> st_wp b)
-  (v : repr a wp_v) (f : (x:a -> repr b (wp_f x)))
-  : repr b (bind_wp wp_v wp_f) =
-  interp_bind v f wp_v wp_f;
-  tbind v f
-
-let subcomp2 (a:Type) (w1 w2: st_wp a)
-  (f : repr a w1)
-  : Pure (repr a w2)
-         (requires w2 `stronger` w1)
-         (ensures fun _ -> True)
-  = f
-
-let if_then_else2 (a : Type) (w1 w2 : st_wp a)
-    (f : repr a w1) (g : repr a w2) (b : bool) : Type =
-  repr a (if b then w1 else w2)
-
-total
-reifiable
-reflectable
-effect {
-  AlgWP (a:Type) (_:st_wp a)
-  with {repr;
-        return = return2;
-        bind   = bind2;
-        subcomp = subcomp2;
-        if_then_else = if_then_else2}
-}
-
-let get2 () : AlgWP state read_wp =
-  AlgWP?.reflect _get
-
-let put2 (s:state) : AlgWP unit (write_wp s) =
-  AlgWP?.reflect (_put s)
-
-open FStar.Monotonic.Pure
-
-unfold
-let lift_pure_wp (#a:Type) (wp : pure_wp a) : st_wp a =
-  elim_pure_wp_monotonicity wp;
-  fun s0 p -> wp (fun x -> p (x, s0))
-
-let lift_pure_algwp (a:Type) wp (f:unit -> PURE a wp)
-  : Pure (repr a (lift_pure_wp wp)) // can't call f() here, so lift its wp instead
-         (requires (wp (fun _ -> True)))
-         (ensures (fun _ -> True))
-  = let v : a = elim_pure f (fun _ -> True) in
-    FStar.Monotonic.Pure.elim_pure_wp_monotonicity wp; // need this lemma
-    assert (forall p. wp p ==> p v); // this is key fact needed for the proof
-    assert_norm (stronger (lift_pure_wp wp) (return_wp v));
-    Return v
-
-sub_effect PURE ~> AlgWP = lift_pure_algwp
-
-let sel (r:loc) : AlgWP int (fun h0 p -> p (Map.sel h0 r, h0)) =
-  let h = get2 () in
-  Map.sel h r
-
-let upd (r:loc) (v:int) : AlgWP unit (fun h0 p -> p ((), Map.upd h0 r v)) =
-  let h = get2 () in
-  put2 (Map.upd h r v)
+let upd (r:loc) (v:int) : tree unit [Read;Write] =
+  let! h = get () in
+  put (Map.upd h r v)
 
 let (!) = sel
 let (:=) = upd
 
-let modifies1 (l:loc) (h0 h1 : state) : prop =
-  forall y. y <> l ==> Map.sel h0 y == Map.sel h1 y
- 
-let modifies (ls: list loc) (h0 h1 : state) : prop = 
-  forall y. mem y ls \/ (Map.sel h0 y == Map.sel h1 y)
+let addx (l:loc) (x:int) : tree unit [Read;Read;Write] =
+  let! v = !l in
+  l := v + x
 
-effect AlgPP (a:Type) (pre : state -> prop) (post : state -> a -> state -> prop) =
-  AlgWP a (fun h0 p -> pre h0 /\ (forall y h1. post h0 y h1 ==> p (y, h1)))
-
-let addx (l:loc) (x:int) : AlgPP unit (fun _ -> True) (fun h0 _ h1 -> modifies1 l h0 h1
-                                                          /\ (Map.sel h1 l == x + Map.sel h0 l)) =
-  l := !l + x
-
-let swap (l1 l2 : loc) : AlgPP unit (fun _ -> l1 <> l2)
-                                    (fun h0 _ h1 -> 
-                                       modifies [l1;l2] h0 h1 /\
-                                       Map.sel h1 l1 == Map.sel h0 l2 /\
-                                       Map.sel h1 l2 == Map.sel h0 l1)
-  =
-  let r = !l2 in
-  l2 := !l1;
-  l1 := r
-
-let rec interp_sem #a (t : rwtree a) (s0:state)
-  : ID5.ID (a & state) (as_pure_wp (interp_as_wp t s0))
-  = match t with
-    | Return x -> (x, s0)
-    | Op Read i k -> 
-      interp_sem (k s0) s0
-    | Op Write i k ->
-      interp_sem (k ()) i
-    
-
-let extract #a #w (c:repr a w)
-  : Lemma (w `stronger` interp_as_wp c)
-  = ()
-
-let soundness_aux #a #wp (t:repr a wp)
-  : Tot (s0:state -> ID5.ID (a & state) (as_pure_wp (wp s0)))
-  = extract t;
-    interp_sem t
-
-let soundness #a #wp (t : unit -> AlgWP a wp)
-  : Tot (s0:state -> ID5.ID (a & state) (as_pure_wp (wp s0)))
-  = soundness_aux (reify (t ()))
-
-(* Same as above, but one doesn't have to think about WPs *)
-let soundnessPP #a #pre #post (t : unit -> AlgPP a pre post)
-  : s0:state{pre s0} -> r:(a & state){post s0 (fst r) (snd r)}
-  = fun s0 -> reify (soundness #a #(fun h0 p -> pre h0 /\ (forall y h1. post h0 y h1 ==> p (y, h1))) t s0)
-                 (fun r -> post s0 (fst r) (snd r))
-                 ()
+let swap (l1 l2 : loc) : tree unit [Read;Read;Read;Write;Read;Write] =
+  let! r1 = !l1 in
+  let! r2 = !l2 in
+  let! _ = l1 := r2 in
+  l2 := r1
