tests/bug-reports/closed/Bug2641.fst
@@ -6,11 +6,15 @@ open FStar.Tactics.Typeclasses
 //
 // Original report by Cezar and Theo
 //
+// The original repro was phrased in terms of an indexed effect FREEwp built
+// from the free monad below.  Indexed effects are gone, so we use the free
+// monad directly (with `let!` notation).
+//
 
 noeq
 type free (a:Type u#a) : Type u#(max a 1) =
 | Return : a -> free a
-| PartialCall : (pre:pure_pre) -> cont:((squash pre) -> free u#a a) -> free a
+| PartialCall : (pre:prop) -> cont:((squash pre) -> free u#a a) -> free a
 
 let rec free_bind (#a:Type u#a) (#b:Type u#b) (l:free a) (k: a -> free b) : free b =
   match l with
@@ -18,9 +22,19 @@ let rec free_bind (#a:Type u#a) (#b:Type u#b) (l:free a) (k: a -> free b) : free
   | PartialCall pre fnc ->
     PartialCall pre (fun _ -> free_bind (fnc ()) k)
 
+let ( let! ) (#a:Type u#a) (#b:Type u#b) (l:free a) (k: a -> free b) : free b =
+  free_bind l k
+
+let partial_call (pre:prop) : free (squash pre) =
+  PartialCall pre (fun x -> Return x)
+
 (** *** Spec **)
+
 (** monotonicity seems relevant **)
-let hist a = wp:(pure_wp' a){pure_wp_monotonic0 a wp}
+let hist_monotonic0 (a:Type) (wp:(a -> prop) -> prop) =
+  forall p1 p2. (forall x. p1 x ==> p2 x) ==> wp p1 ==> wp p2
+
+let hist a = wp:((a -> prop) -> prop){hist_monotonic0 a wp}
 
 val hist_ord (#a : Type) : hist a -> hist a -> prop
 let hist_ord wp1 wp2 = forall p. wp1 p ==> wp2 p
@@ -31,30 +45,25 @@ let hist_return (x:'a) : hist 'a =
 let hist_bind (#a #b:Type) (w : hist a) (kw : a -> hist b) : hist b =
   fun p -> w (fun r -> kw r p)
 
-let wp_lift_pure_hist (#a:Type u#a) (w : pure_wp a) : hist a =
-  FStar.Monotonic.Pure.elim_pure_wp_monotonicity_forall u#a ();
-  w
+let partial_call_wp (pre:prop) : hist (squash pre) =
+  fun p -> pre /\ p ()
 
-let partial_call_wp (pre:pure_pre) : hist (squash pre) = 
-  let wp' : pure_wp' (squash pre) = fun p -> pre /\ p () in
-  wp'
+(** *** Effect observation **)
 
-
-(** *** Dijkstra Monad **)
 val theta : #a:Type -> free a -> hist a
 let rec theta m =
   match m with
   | Return x -> hist_return x
-  | PartialCall pre k -> 
+  | PartialCall pre k ->
     hist_bind (partial_call_wp pre) (fun r -> theta (k r))
 
 let dm_free (a:Type) (wp:hist a) =
-  tree:(free a){wp `hist_ord` theta tree} 
+  tree:(free a){wp `hist_ord` theta tree}
 
 val dm_free_return : (a:Type) -> (x:a) -> dm_free a (hist_return x)
 let dm_free_return a x = Return x
 
-val lemma_monad_morphism  : 
+val lemma_monad_morphism  :
   a: Type ->
   b: Type ->
   v: free a ->
@@ -63,14 +72,14 @@ val lemma_monad_morphism  :
 let rec lemma_monad_morphism a b v f =
   match v with
   | Return _ -> ()
-  | PartialCall pre k -> 
+  | PartialCall pre k ->
     calc (hist_ord) {
       hist_bind (theta (PartialCall pre k)) (fun x -> theta (f x));
       == { _ by (FStar.Tactics.compute ()) }
       hist_bind (hist_bind (partial_call_wp pre) (fun r -> theta (k r))) (fun x -> theta (f x));
       == { _ by (FStar.Tactics.compute ()) }
       hist_bind (partial_call_wp pre) (fun r -> hist_bind (theta (k r)) (fun x -> theta (f x)));
-      `hist_ord` {         
+      `hist_ord` {
         let rhs1 : squash pre -> hist b = fun r -> hist_bind (theta (k r)) (fun x -> theta (f x)) in
         let rhs2 : squash pre -> hist b = fun r -> theta (free_bind (k r) f) in
         introduce forall (r:squash pre). (rhs1 r) `hist_ord` (rhs2 r) with begin
@@ -81,8 +90,8 @@ let rec lemma_monad_morphism a b v f =
       `hist_ord` { _ by (FStar.Tactics.compute ()) }
       theta (free_bind (PartialCall pre k) f);
     }
-  
-val dm_free_bind  : 
+
+val dm_free_bind  :
   a: Type ->
   b: Type ->
   wp_v: hist a ->
@@ -94,37 +103,13 @@ let dm_free_bind a b wp_v wp_f v f =
   lemma_monad_morphism a b v f;
   free_bind v f
 
-val dm_free_subcomp : 
+val dm_free_subcomp :
   a: Type ->
   wp1: hist a ->
   wp2: hist a ->
   f: dm_free a wp1 ->
   Pure (dm_free a wp2) (hist_ord wp2 wp1) (fun _ -> True)
 let dm_free_subcomp a wp1 wp2 f = f
-
-val lift_pure_dm_free :
-  a: Type ->
-  w: pure_wp a ->
-  f: (_: unit -> PURE a w) ->
-  Tot (dm_free a (wp_lift_pure_hist w))
-let lift_pure_dm_free a w f =
-  FStar.Monotonic.Pure.elim_pure_wp_monotonicity_forall ();
-  PartialCall (as_requires w) (fun proof -> Return (f proof))
-
-total
-reifiable
-reflectable
-effect {
-  FREEwp (a:Type) (wp : hist a) 
-  with {
-       repr       = dm_free
-     ; return     = dm_free_return
-     ; bind       = dm_free_bind 
-     ; subcomp    = dm_free_subcomp
-     }
-}
-
-sub_effect PURE ~> FREEwp = lift_pure_dm_free
 
 class compilable (t:Type) = {
   comp_type : Type;
@@ -143,13 +128,13 @@ instance compile_option (t:Type) {| d1:compilable t |} : compilable (option t) =
 let test_assert_false
   (t1:Type)
   (t2:Type)
-  {| d2:compilable t2 |} 
-  (f:(t1 -> FREEwp (option t2) (fun p -> (forall r. p r)))) 
-  (x:t1) : 
+  {| d2:compilable t2 |}
+  (f:(t1 -> free (option t2)))
+  (x:t1) :
   Lemma False =
   let _ : dm_free (option d2.comp_type) (hist_bind (fun p -> forall r . p r)
                                                    (fun (r:option t2) -> hist_return (compile #(option t2) #(compile_option t2 #d2) r))) =
-       reify (compile #(option t2) #(compile_option t2 #d2) (f x)) in
+       (let! v = f x in Return (compile #(option t2) #(compile_option t2 #d2) v)) in
   assert (False)
 
 
@@ -163,11 +148,11 @@ let compile_option2 : (option int -> option int) =
         | Some r -> Some r
 
 [@@ expect_failure [19]]
-let test_assert_false
-  (f:(unit -> FREEwp (option int) (fun p -> (forall r. p r)))) : 
+let test_assert_false2
+  (f:(unit -> free (option int))) :
   Lemma False =
   let _ : dm_free (option int) (hist_bind (fun p -> forall r . p r)
                                         (fun (r:option int) -> hist_return ((compile_option2 r)))) =
-       reify (let eff_val = f () in
-              compile_option2 eff_val) in
+       (let! eff_val = f () in
+        Return (compile_option2 eff_val)) in
   assert False
