ulib/FStar.Exn.fst
@@ -19,5 +19,5 @@ module FStar.Exn
 (** Providing the signature of [raise],
     that is implemented natively in FStar_Exn.ml as primitive raise *)
 assume
-val raise (e: exn) : Exn 'a (requires True) (ensures (fun r -> r == E e))
+val raise (e: exn) : Exn 'a (ensures fun _ -> False)
 
